Flean/StorageFormats.lean
@@ -3,3 +3,4 @@ import Flean.StorageFormats.Conversion
 import Flean.StorageFormats.FromFp
 import Flean.StorageFormats.RoundRNEVerify
 import Flean.StorageFormats.RoundTrip
+import Flean.StorageFormats.FromFpCorrect
